<?xml version="1.0"?>


<!DOCTYPE rdf:RDF [
    <!ENTITY owl "http://www.w3.org/2002/07/owl#" >
    <!ENTITY xsd "http://www.w3.org/2001/XMLSchema#" >
    <!ENTITY rdfs "http://www.w3.org/2000/01/rdf-schema#" >
    <!ENTITY rdf "http://www.w3.org/1999/02/22-rdf-syntax-ns#" >
]>


<rdf:RDF xmlns="http://www.semanticweb.org/nalkhald/ontologies/2016/3/untitled-ontology-3#"
     xml:base="http://www.semanticweb.org/nalkhald/ontologies/2016/3/untitled-ontology-3"
     xmlns:rdfs="http://www.w3.org/2000/01/rdf-schema#"
     xmlns:owl="http://www.w3.org/2002/07/owl#"
     xmlns:xsd="http://www.w3.org/2001/XMLSchema#"
     xmlns:rdf="http://www.w3.org/1999/02/22-rdf-syntax-ns#">
    <owl:Ontology rdf:about="http://www.semanticweb.org/nalkhald/ontologies/2016/3/untitled-ontology-3">
        <owl:imports rdf:resource="http://www.mis.ugent.be/ontologies/ufo.owl"/>
    </owl:Ontology>
    


    <!-- 
    ///////////////////////////////////////////////////////////////////////////////////////
    //
    // Classes
    //
    ///////////////////////////////////////////////////////////////////////////////////////
     -->

    


    <!-- http://www.semanticweb.org/nalkhald/ontologies/2016/3/untitled-ontology-3#Administrative -->

    <owl:Class rdf:about="http://www.semanticweb.org/nalkhald/ontologies/2016/3/untitled-ontology-3#Administrative">
        <rdfs:subClassOf rdf:resource="http://www.semanticweb.org/nalkhald/ontologies/2016/3/untitled-ontology-3#Person"/>
        <rdfs:comment>An employee responsible for administrative tasks</rdfs:comment>
    </owl:Class>
    


    <!-- http://www.semanticweb.org/nalkhald/ontologies/2016/3/untitled-ontology-3#Appy_Treatment -->

    <owl:Class rdf:about="http://www.semanticweb.org/nalkhald/ontologies/2016/3/untitled-ontology-3#Appy_Treatment"/>
    


    <!-- http://www.semanticweb.org/nalkhald/ontologies/2016/3/untitled-ontology-3#BloodPressure -->

    <owl:Class rdf:about="http://www.semanticweb.org/nalkhald/ontologies/2016/3/untitled-ontology-3#BloodPressure">
        <rdfs:subClassOf rdf:resource="http://www.semanticweb.org/nalkhald/ontologies/2016/3/untitled-ontology-3#VitalSigns"/>
        <rdfs:comment>The pressure of the blood in the circulatory system, 
often measured for diagnosis  as it is closely related 
to the force and rate of the heartbeat and the 
diameter and elasticity of the arteria walls.</rdfs:comment>
    </owl:Class>
    


    <!-- http://www.semanticweb.org/nalkhald/ontologies/2016/3/untitled-ontology-3#Clinic -->

    <owl:Class rdf:about="http://www.semanticweb.org/nalkhald/ontologies/2016/3/untitled-ontology-3#Clinic">
        <rdfs:comment>An establishment where patients are admitted 
for special study and treatment by a group of 
health care professionals practicing together</rdfs:comment>
    </owl:Class>
    


    <!-- http://www.semanticweb.org/nalkhald/ontologies/2016/3/untitled-ontology-3#ClinicalInitiativeNurse -->

    <owl:Class rdf:about="http://www.semanticweb.org/nalkhald/ontologies/2016/3/untitled-ontology-3#ClinicalInitiativeNurse">
        <rdfs:subClassOf rdf:resource="http://www.semanticweb.org/nalkhald/ontologies/2016/3/untitled-ontology-3#ClinicalStaff"/>
        <rdfs:comment>A nurse who is providing nursing care 
to patients in emergency department&apos;s 
waiting room</rdfs:comment>
    </owl:Class>
    


    <!-- http://www.semanticweb.org/nalkhald/ontologies/2016/3/untitled-ontology-3#ClinicalStaff -->

    <owl:Class rdf:about="http://www.semanticweb.org/nalkhald/ontologies/2016/3/untitled-ontology-3#ClinicalStaff">
        <rdfs:subClassOf rdf:resource="http://www.semanticweb.org/nalkhald/ontologies/2016/3/untitled-ontology-3#Person"/>
        <rdfs:comment>A person who works under the supervision 
of a physician or other qualified health care 
professional and who is allowed by law, 
regulations and facility policy to perform or 
assist in performance of a specified 
professional service</rdfs:comment>
    </owl:Class>
    


    <!-- http://www.semanticweb.org/nalkhald/ontologies/2016/3/untitled-ontology-3#Condition -->

    <owl:Class rdf:about="http://www.semanticweb.org/nalkhald/ontologies/2016/3/untitled-ontology-3#Condition"/>
    


    <!-- http://www.semanticweb.org/nalkhald/ontologies/2016/3/untitled-ontology-3#Cough -->

    <owl:Class rdf:about="http://www.semanticweb.org/nalkhald/ontologies/2016/3/untitled-ontology-3#Cough">
        <rdfs:subClassOf rdf:resource="http://www.semanticweb.org/nalkhald/ontologies/2016/3/untitled-ontology-3#Symptoms"/>
        <rdfs:comment>Cough is a natural reflex that protects the lungs. 
Coughing helps to clear the airways of lung irritants 
such as smoke and mucus.  This helps to prevent 
infections. A cough is also a symptom of a medical problem</rdfs:comment>
    </owl:Class>
    


    <!-- http://www.semanticweb.org/nalkhald/ontologies/2016/3/untitled-ontology-3#Data -->

    <owl:Class rdf:about="http://www.semanticweb.org/nalkhald/ontologies/2016/3/untitled-ontology-3#Data">
        <rdfs:comment>Piece of information which is a part of a collection to be used in an analyses of a problem, such as diagnosis of a health problem.</rdfs:comment>
    </owl:Class>
    


    <!-- http://www.semanticweb.org/nalkhald/ontologies/2016/3/untitled-ontology-3#Device -->

    <owl:Class rdf:about="http://www.semanticweb.org/nalkhald/ontologies/2016/3/untitled-ontology-3#Device">
        <rdfs:comment>An appliance, usually mechanical, designed to perform a specific function.</rdfs:comment>
    </owl:Class>
    


    <!-- http://www.semanticweb.org/nalkhald/ontologies/2016/3/untitled-ontology-3#Diagnosis -->

    <owl:Class rdf:about="http://www.semanticweb.org/nalkhald/ontologies/2016/3/untitled-ontology-3#Diagnosis">
        <rdfs:comment>Determination of the nature of the cause of a disease.</rdfs:comment>
    </owl:Class>
    


    <!-- http://www.semanticweb.org/nalkhald/ontologies/2016/3/untitled-ontology-3#DifferentialDiagnosis -->

    <owl:Class rdf:about="http://www.semanticweb.org/nalkhald/ontologies/2016/3/untitled-ontology-3#DifferentialDiagnosis">
        <rdfs:subClassOf rdf:resource="http://www.semanticweb.org/nalkhald/ontologies/2016/3/untitled-ontology-3#Diagnosis"/>
        <rdfs:comment>The determination which one of the several 
diseases may be producing the symptoms</rdfs:comment>
    </owl:Class>
    


    <!-- http://www.semanticweb.org/nalkhald/ontologies/2016/3/untitled-ontology-3#EmergencyDepartment -->

    <owl:Class rdf:about="http://www.semanticweb.org/nalkhald/ontologies/2016/3/untitled-ontology-3#EmergencyDepartment">
        <rdfs:comment>A section of an institution that is staffed 
and equipped to provide rapid and varied 
emergency care, specially for those who 
are stricken with sudden and acute illness 
or who are victims of severe trauma</rdfs:comment>
    </owl:Class>
    


    <!-- http://www.semanticweb.org/nalkhald/ontologies/2016/3/untitled-ontology-3#Examination -->

    <owl:Class rdf:about="http://www.semanticweb.org/nalkhald/ontologies/2016/3/untitled-ontology-3#Examination">
        <rdfs:comment>Examination of body state, made for the purpose of diagnosis.</rdfs:comment>
    </owl:Class>
    


    <!-- http://www.semanticweb.org/nalkhald/ontologies/2016/3/untitled-ontology-3#Examine_Symptoms -->

    <owl:Class rdf:about="http://www.semanticweb.org/nalkhald/ontologies/2016/3/untitled-ontology-3#Examine_Symptoms">
        <rdfs:subClassOf rdf:resource="http://www.semanticweb.org/nalkhald/ontologies/2016/3/untitled-ontology-3#Perform_Examination"/>
    </owl:Class>
    


    <!-- http://www.semanticweb.org/nalkhald/ontologies/2016/3/untitled-ontology-3#Fever -->

    <owl:Class rdf:about="http://www.semanticweb.org/nalkhald/ontologies/2016/3/untitled-ontology-3#Fever">
        <rdfs:subClassOf rdf:resource="http://www.semanticweb.org/nalkhald/ontologies/2016/3/untitled-ontology-3#Symptoms"/>
        <rdfs:comment>Is body temperature elivation over 37.8 degree Celsuis</rdfs:comment>
    </owl:Class>
    


    <!-- http://www.semanticweb.org/nalkhald/ontologies/2016/3/untitled-ontology-3#Headache -->

    <owl:Class rdf:about="http://www.semanticweb.org/nalkhald/ontologies/2016/3/untitled-ontology-3#Headache">
        <rdfs:subClassOf rdf:resource="http://www.semanticweb.org/nalkhald/ontologies/2016/3/untitled-ontology-3#Symptoms"/>
        <rdfs:comment>A headache involves pain in the head 
which can arise from many disorders 
or may be a disorder of itself</rdfs:comment>
    </owl:Class>
    


    <!-- http://www.semanticweb.org/nalkhald/ontologies/2016/3/untitled-ontology-3#HealthCare -->

    <owl:Class rdf:about="http://www.semanticweb.org/nalkhald/ontologies/2016/3/untitled-ontology-3#HealthCare">
        <rdfs:comment>Health care provided by a medical facility to a patient</rdfs:comment>
    </owl:Class>
    


    <!-- http://www.semanticweb.org/nalkhald/ontologies/2016/3/untitled-ontology-3#HeartBeat -->

    <owl:Class rdf:about="http://www.semanticweb.org/nalkhald/ontologies/2016/3/untitled-ontology-3#HeartBeat">
        <rdfs:subClassOf rdf:resource="http://www.semanticweb.org/nalkhald/ontologies/2016/3/untitled-ontology-3#VitalSigns"/>
        <rdfs:comment>A complete cardiac cycle, including spread 
of the electrical impulse and a consequent 
mechanical contraction</rdfs:comment>
    </owl:Class>
    


    <!-- http://www.semanticweb.org/nalkhald/ontologies/2016/3/untitled-ontology-3#HearthAttack -->

    <owl:Class rdf:about="http://www.semanticweb.org/nalkhald/ontologies/2016/3/untitled-ontology-3#HearthAttack"/>
    


    <!-- http://www.semanticweb.org/nalkhald/ontologies/2016/3/untitled-ontology-3#Hospital -->

    <owl:Class rdf:about="http://www.semanticweb.org/nalkhald/ontologies/2016/3/untitled-ontology-3#Hospital">
        <rdfs:comment>An institution for the care and treatment 
of the acutely sick and injured</rdfs:comment>
    </owl:Class>
    


    <!-- http://www.semanticweb.org/nalkhald/ontologies/2016/3/untitled-ontology-3#IDCard -->

    <owl:Class rdf:about="http://www.semanticweb.org/nalkhald/ontologies/2016/3/untitled-ontology-3#IDCard">
        <rdfs:subClassOf rdf:resource="http://www.semanticweb.org/nalkhald/ontologies/2016/3/untitled-ontology-3#Data"/>
        <rdfs:comment>Is a cocument which may be used to identify a person, or verify aspects of a person&apos;s personal identity</rdfs:comment>
    </owl:Class>
    


    <!-- http://www.semanticweb.org/nalkhald/ontologies/2016/3/untitled-ontology-3#MedicalFacility -->

    <owl:Class rdf:about="http://www.semanticweb.org/nalkhald/ontologies/2016/3/untitled-ontology-3#MedicalFacility">
        <rdfs:comment>Health care institution which have accommodation facilities, and which engage in providing short -term and long - term medical treatment of a general or specialized nature</rdfs:comment>
    </owl:Class>
    


    <!-- http://www.semanticweb.org/nalkhald/ontologies/2016/3/untitled-ontology-3#MedicalHistory -->

    <owl:Class rdf:about="http://www.semanticweb.org/nalkhald/ontologies/2016/3/untitled-ontology-3#MedicalHistory">
        <rdfs:subClassOf rdf:resource="http://www.semanticweb.org/nalkhald/ontologies/2016/3/untitled-ontology-3#Data"/>
        <rdfs:comment>Information about the medical history
of a patient</rdfs:comment>
    </owl:Class>
    


    <!-- http://www.semanticweb.org/nalkhald/ontologies/2016/3/untitled-ontology-3#MedicalInstitution -->

    <owl:Class rdf:about="http://www.semanticweb.org/nalkhald/ontologies/2016/3/untitled-ontology-3#MedicalInstitution">
        <rdfs:comment>Any public or private, medical or dental facility where clinical trials are conducted.</rdfs:comment>
    </owl:Class>
    


    <!-- http://www.semanticweb.org/nalkhald/ontologies/2016/3/untitled-ontology-3#Medication -->

    <owl:Class rdf:about="http://www.semanticweb.org/nalkhald/ontologies/2016/3/untitled-ontology-3#Medication">
        <rdfs:comment>Any Chemical compound used in diagnosis, treatment or prevention of desease or other abnormal condition</rdfs:comment>
    </owl:Class>
    


    <!-- http://www.semanticweb.org/nalkhald/ontologies/2016/3/untitled-ontology-3#Paramedics -->

    <owl:Class rdf:about="http://www.semanticweb.org/nalkhald/ontologies/2016/3/untitled-ontology-3#Paramedics">
        <rdfs:subClassOf rdf:resource="http://www.semanticweb.org/nalkhald/ontologies/2016/3/untitled-ontology-3#Person"/>
        <rdfs:comment>A person who is trained to do medical work, 
specially emergency first aid, but is not a full 
qualified doctor</rdfs:comment>
    </owl:Class>
    


    <!-- http://www.semanticweb.org/nalkhald/ontologies/2016/3/untitled-ontology-3#Passport -->

    <owl:Class rdf:about="http://www.semanticweb.org/nalkhald/ontologies/2016/3/untitled-ontology-3#Passport">
        <rdfs:subClassOf rdf:resource="http://www.semanticweb.org/nalkhald/ontologies/2016/3/untitled-ontology-3#Data"/>
        <rdfs:comment>An official document issued by a government, certifying holder&apos;s identity and citizenship, and entiteling them to travel under its protection to and from foreign countries.</rdfs:comment>
    </owl:Class>
    


    <!-- http://www.semanticweb.org/nalkhald/ontologies/2016/3/untitled-ontology-3#Patient -->

    <owl:Class rdf:about="http://www.semanticweb.org/nalkhald/ontologies/2016/3/untitled-ontology-3#Patient">
        <rdfs:subClassOf rdf:resource="http://www.semanticweb.org/nalkhald/ontologies/2016/3/untitled-ontology-3#Person"/>
        <rdfs:comment>A person who is ill or is undergoing treatment for disease.</rdfs:comment>
    </owl:Class>
    


    <!-- http://www.semanticweb.org/nalkhald/ontologies/2016/3/untitled-ontology-3#PatientArrived -->

    <owl:Class rdf:about="http://www.semanticweb.org/nalkhald/ontologies/2016/3/untitled-ontology-3#PatientArrived">
        <rdfs:comment>An event indicating patient&apos;s arrival to the medical facility</rdfs:comment>
    </owl:Class>
    


    <!-- http://www.semanticweb.org/nalkhald/ontologies/2016/3/untitled-ontology-3#PatientDischarged -->

    <owl:Class rdf:about="http://www.semanticweb.org/nalkhald/ontologies/2016/3/untitled-ontology-3#PatientDischarged">
        <rdfs:comment>An event indicating that the patient was discharged from the medical facility</rdfs:comment>
    </owl:Class>
    


    <!-- http://www.semanticweb.org/nalkhald/ontologies/2016/3/untitled-ontology-3#PatientRedirected -->

    <owl:Class rdf:about="http://www.semanticweb.org/nalkhald/ontologies/2016/3/untitled-ontology-3#PatientRedirected">
        <rdfs:comment>An event indicating that the patient was redirected to another medical facility</rdfs:comment>
    </owl:Class>
    


    <!-- http://www.semanticweb.org/nalkhald/ontologies/2016/3/untitled-ontology-3#PediatricServices -->

    <owl:Class rdf:about="http://www.semanticweb.org/nalkhald/ontologies/2016/3/untitled-ontology-3#PediatricServices">
        <rdfs:comment>Medical services offered to infants, children and adolescents</rdfs:comment>
    </owl:Class>
    


    <!-- http://www.semanticweb.org/nalkhald/ontologies/2016/3/untitled-ontology-3#Perform_Examination -->

    <owl:Class rdf:about="http://www.semanticweb.org/nalkhald/ontologies/2016/3/untitled-ontology-3#Perform_Examination"/>
    


    <!-- http://www.semanticweb.org/nalkhald/ontologies/2016/3/untitled-ontology-3#Perform_PhysicalExamination -->

    <owl:Class rdf:about="http://www.semanticweb.org/nalkhald/ontologies/2016/3/untitled-ontology-3#Perform_PhysicalExamination">
        <rdfs:subClassOf rdf:resource="http://www.semanticweb.org/nalkhald/ontologies/2016/3/untitled-ontology-3#Perform_Examination"/>
    </owl:Class>
    


    <!-- http://www.semanticweb.org/nalkhald/ontologies/2016/3/untitled-ontology-3#Perform_SurgicalExamination -->

    <owl:Class rdf:about="http://www.semanticweb.org/nalkhald/ontologies/2016/3/untitled-ontology-3#Perform_SurgicalExamination">
        <rdfs:subClassOf rdf:resource="http://www.semanticweb.org/nalkhald/ontologies/2016/3/untitled-ontology-3#Perform_Examination"/>
        <rdfs:comment>Examination performed by a Surgeon</rdfs:comment>
    </owl:Class>
    


    <!-- http://www.semanticweb.org/nalkhald/ontologies/2016/3/untitled-ontology-3#Person -->

    <owl:Class rdf:about="http://www.semanticweb.org/nalkhald/ontologies/2016/3/untitled-ontology-3#Person">
        <rdfs:comment>A living human</rdfs:comment>
    </owl:Class>
    


    <!-- http://www.semanticweb.org/nalkhald/ontologies/2016/3/untitled-ontology-3#Pharmacy -->

    <owl:Class rdf:about="http://www.semanticweb.org/nalkhald/ontologies/2016/3/untitled-ontology-3#Pharmacy">
        <rdfs:comment>A place where drugs are compounded or dispensed</rdfs:comment>
    </owl:Class>
    


    <!-- http://www.semanticweb.org/nalkhald/ontologies/2016/3/untitled-ontology-3#PhysicalExamination -->

    <owl:Class rdf:about="http://www.semanticweb.org/nalkhald/ontologies/2016/3/untitled-ontology-3#PhysicalExamination">
        <rdfs:subClassOf rdf:resource="http://www.semanticweb.org/nalkhald/ontologies/2016/3/untitled-ontology-3#Examination"/>
        <rdfs:comment>Examination of body state, made for the purpose of diagnosis.</rdfs:comment>
    </owl:Class>
    


    <!-- http://www.semanticweb.org/nalkhald/ontologies/2016/3/untitled-ontology-3#PhysicalTherapy -->

    <owl:Class rdf:about="http://www.semanticweb.org/nalkhald/ontologies/2016/3/untitled-ontology-3#PhysicalTherapy">
        <rdfs:subClassOf rdf:resource="http://www.semanticweb.org/nalkhald/ontologies/2016/3/untitled-ontology-3#Therapy"/>
        <rdfs:comment>Treatment in order to prevent, correct, 
and limit physical disability and bodily malfuntioning</rdfs:comment>
    </owl:Class>
    


    <!-- http://www.semanticweb.org/nalkhald/ontologies/2016/3/untitled-ontology-3#Physician -->

    <owl:Class rdf:about="http://www.semanticweb.org/nalkhald/ontologies/2016/3/untitled-ontology-3#Physician">
        <rdfs:subClassOf rdf:resource="http://www.semanticweb.org/nalkhald/ontologies/2016/3/untitled-ontology-3#Person"/>
        <rdfs:comment>An authorized practitioner of medicine, 
as one graduated from a college of medicine 
and licensed by the appropriate board</rdfs:comment>
    </owl:Class>
    


    <!-- http://www.semanticweb.org/nalkhald/ontologies/2016/3/untitled-ontology-3#Radiation -->

    <owl:Class rdf:about="http://www.semanticweb.org/nalkhald/ontologies/2016/3/untitled-ontology-3#Radiation">
        <rdfs:subClassOf rdf:resource="http://www.semanticweb.org/nalkhald/ontologies/2016/3/untitled-ontology-3#Therapy"/>
        <rdfs:comment>Application of x-ray or radioactive 
substances for treatment of various illnesses</rdfs:comment>
    </owl:Class>
    


    <!-- http://www.semanticweb.org/nalkhald/ontologies/2016/3/untitled-ontology-3#SpeachTherapy -->

    <owl:Class rdf:about="http://www.semanticweb.org/nalkhald/ontologies/2016/3/untitled-ontology-3#SpeachTherapy">
        <rdfs:subClassOf rdf:resource="http://www.semanticweb.org/nalkhald/ontologies/2016/3/untitled-ontology-3#Therapy"/>
        <rdfs:comment>Training to help people with speech and language problems.</rdfs:comment>
    </owl:Class>
    


    <!-- http://www.semanticweb.org/nalkhald/ontologies/2016/3/untitled-ontology-3#Surgeon -->

    <owl:Class rdf:about="http://www.semanticweb.org/nalkhald/ontologies/2016/3/untitled-ontology-3#Surgeon">
        <rdfs:subClassOf rdf:resource="http://www.semanticweb.org/nalkhald/ontologies/2016/3/untitled-ontology-3#Physician"/>
        <rdfs:comment>A doctor specialized in surgery</rdfs:comment>
    </owl:Class>
    


    <!-- http://www.semanticweb.org/nalkhald/ontologies/2016/3/untitled-ontology-3#Surgery -->

    <owl:Class rdf:about="http://www.semanticweb.org/nalkhald/ontologies/2016/3/untitled-ontology-3#Surgery">
        <rdfs:subClassOf rdf:resource="http://www.semanticweb.org/nalkhald/ontologies/2016/3/untitled-ontology-3#Therapy"/>
        <rdfs:comment>Operation performed by a qualified surgeon 
for removal or replacement of a diseased 
tissue by cutting</rdfs:comment>
    </owl:Class>
    


    <!-- http://www.semanticweb.org/nalkhald/ontologies/2016/3/untitled-ontology-3#Symptoms -->

    <owl:Class rdf:about="http://www.semanticweb.org/nalkhald/ontologies/2016/3/untitled-ontology-3#Symptoms">
        <rdfs:comment>Subjective indication of a disease 
or a change in condition as 
perceived by the patient</rdfs:comment>
    </owl:Class>
    


    <!-- http://www.semanticweb.org/nalkhald/ontologies/2016/3/untitled-ontology-3#Therapy -->

    <owl:Class rdf:about="http://www.semanticweb.org/nalkhald/ontologies/2016/3/untitled-ontology-3#Therapy">
        <rdfs:comment>Treatment of disease or disorder by any method</rdfs:comment>
    </owl:Class>
    


    <!-- http://www.semanticweb.org/nalkhald/ontologies/2016/3/untitled-ontology-3#Trauma -->

    <owl:Class rdf:about="http://www.semanticweb.org/nalkhald/ontologies/2016/3/untitled-ontology-3#Trauma">
        <rdfs:subClassOf rdf:resource="http://www.semanticweb.org/nalkhald/ontologies/2016/3/untitled-ontology-3#Symptoms"/>
        <rdfs:comment>Injury, psychological or emotional damage</rdfs:comment>
    </owl:Class>
    


    <!-- http://www.semanticweb.org/nalkhald/ontologies/2016/3/untitled-ontology-3#Treatment -->

    <owl:Class rdf:about="http://www.semanticweb.org/nalkhald/ontologies/2016/3/untitled-ontology-3#Treatment">
        <rdfs:comment>MAnagement and care of the patient</rdfs:comment>
    </owl:Class>
    


    <!-- http://www.semanticweb.org/nalkhald/ontologies/2016/3/untitled-ontology-3#TriageNurse -->

    <owl:Class rdf:about="http://www.semanticweb.org/nalkhald/ontologies/2016/3/untitled-ontology-3#TriageNurse">
        <rdfs:subClassOf rdf:resource="http://www.semanticweb.org/nalkhald/ontologies/2016/3/untitled-ontology-3#ClinicalStaff"/>
        <rdfs:comment>A nurse whose responsibility is sorting patients 
arriving to the emergency department into groups 
based on their need for immediate medical treatment</rdfs:comment>
    </owl:Class>
    


    <!-- http://www.semanticweb.org/nalkhald/ontologies/2016/3/untitled-ontology-3#VitalSigns -->

    <owl:Class rdf:about="http://www.semanticweb.org/nalkhald/ontologies/2016/3/untitled-ontology-3#VitalSigns">
        <rdfs:subClassOf rdf:resource="http://www.semanticweb.org/nalkhald/ontologies/2016/3/untitled-ontology-3#Data"/>
        <rdfs:comment>Measurement of pulse rate, body temperature,
and blood pressure to assess health or disfunction</rdfs:comment>
    </owl:Class>
    


    <!-- 
    ///////////////////////////////////////////////////////////////////////////////////////
    //
    // Individuals
    //
    ///////////////////////////////////////////////////////////////////////////////////////
     -->

    


    <!-- http://www.semanticweb.org/nalkhald/ontologies/2016/3/untitled-ontology-3#Administrative -->

    <owl:NamedIndividual rdf:about="http://www.semanticweb.org/nalkhald/ontologies/2016/3/untitled-ontology-3#Administrative">
        <rdf:type rdf:resource="http://www.mis.ugent.be/ontologies/ufo.owl#Role_Type"/>
    </owl:NamedIndividual>
    


    <!-- http://www.semanticweb.org/nalkhald/ontologies/2016/3/untitled-ontology-3#Apply_Treatment -->

    <owl:NamedIndividual rdf:about="http://www.semanticweb.org/nalkhald/ontologies/2016/3/untitled-ontology-3#Apply_Treatment">
        <rdf:type rdf:resource="http://www.mis.ugent.be/ontologies/ufo.owl#Event_Type"/>
    </owl:NamedIndividual>
    


    <!-- http://www.semanticweb.org/nalkhald/ontologies/2016/3/untitled-ontology-3#BloodPressure -->

    <owl:NamedIndividual rdf:about="http://www.semanticweb.org/nalkhald/ontologies/2016/3/untitled-ontology-3#BloodPressure">
        <rdf:type rdf:resource="http://www.mis.ugent.be/ontologies/ufo.owl#Quality_Universal"/>
    </owl:NamedIndividual>
    


    <!-- http://www.semanticweb.org/nalkhald/ontologies/2016/3/untitled-ontology-3#BodyTemperature -->

    <owl:NamedIndividual rdf:about="http://www.semanticweb.org/nalkhald/ontologies/2016/3/untitled-ontology-3#BodyTemperature">
        <rdf:type rdf:resource="http://www.mis.ugent.be/ontologies/ufo.owl#Quality_Universal"/>
        <rdfs:comment>Measure of the body&apos;s ebility 
to generate and get rid of heat</rdfs:comment>
    </owl:NamedIndividual>
    


    <!-- http://www.semanticweb.org/nalkhald/ontologies/2016/3/untitled-ontology-3#Clinic -->

    <owl:NamedIndividual rdf:about="http://www.semanticweb.org/nalkhald/ontologies/2016/3/untitled-ontology-3#Clinic">
        <rdf:type rdf:resource="http://www.mis.ugent.be/ontologies/ufo.owl#Base_Type"/>
    </owl:NamedIndividual>
    


    <!-- http://www.semanticweb.org/nalkhald/ontologies/2016/3/untitled-ontology-3#ClinicalInitiativeNurse -->

    <owl:NamedIndividual rdf:about="http://www.semanticweb.org/nalkhald/ontologies/2016/3/untitled-ontology-3#ClinicalInitiativeNurse">
        <rdf:type rdf:resource="http://www.mis.ugent.be/ontologies/ufo.owl#Role_Type"/>
    </owl:NamedIndividual>
    


    <!-- http://www.semanticweb.org/nalkhald/ontologies/2016/3/untitled-ontology-3#ClinicalStaff -->

    <owl:NamedIndividual rdf:about="http://www.semanticweb.org/nalkhald/ontologies/2016/3/untitled-ontology-3#ClinicalStaff">
        <rdf:type rdf:resource="http://www.mis.ugent.be/ontologies/ufo.owl#Role_Type"/>
    </owl:NamedIndividual>
    


    <!-- http://www.semanticweb.org/nalkhald/ontologies/2016/3/untitled-ontology-3#Condition -->

    <owl:NamedIndividual rdf:about="http://www.semanticweb.org/nalkhald/ontologies/2016/3/untitled-ontology-3#Condition">
        <rdf:type rdf:resource="http://www.mis.ugent.be/ontologies/ufo.owl#Quality_Universal"/>
    </owl:NamedIndividual>
    


    <!-- http://www.semanticweb.org/nalkhald/ontologies/2016/3/untitled-ontology-3#Cough -->

    <owl:NamedIndividual rdf:about="http://www.semanticweb.org/nalkhald/ontologies/2016/3/untitled-ontology-3#Cough">
        <rdf:type rdf:resource="http://www.mis.ugent.be/ontologies/ufo.owl#Quality_Universal"/>
    </owl:NamedIndividual>
    


    <!-- http://www.semanticweb.org/nalkhald/ontologies/2016/3/untitled-ontology-3#Data -->

    <owl:NamedIndividual rdf:about="http://www.semanticweb.org/nalkhald/ontologies/2016/3/untitled-ontology-3#Data">
        <rdf:type rdf:resource="http://www.mis.ugent.be/ontologies/ufo.owl#Mixin_Type"/>
    </owl:NamedIndividual>
    


    <!-- http://www.semanticweb.org/nalkhald/ontologies/2016/3/untitled-ontology-3#Device -->

    <owl:NamedIndividual rdf:about="http://www.semanticweb.org/nalkhald/ontologies/2016/3/untitled-ontology-3#Device">
        <rdf:type rdf:resource="http://www.mis.ugent.be/ontologies/ufo.owl#Mixin_Type"/>
    </owl:NamedIndividual>
    


    <!-- http://www.semanticweb.org/nalkhald/ontologies/2016/3/untitled-ontology-3#Diagnosis -->

    <owl:NamedIndividual rdf:about="http://www.semanticweb.org/nalkhald/ontologies/2016/3/untitled-ontology-3#Diagnosis">
        <rdf:type rdf:resource="http://www.mis.ugent.be/ontologies/ufo.owl#Quality_Universal"/>
    </owl:NamedIndividual>
    


    <!-- http://www.semanticweb.org/nalkhald/ontologies/2016/3/untitled-ontology-3#DifferentialDiagnosis -->

    <owl:NamedIndividual rdf:about="http://www.semanticweb.org/nalkhald/ontologies/2016/3/untitled-ontology-3#DifferentialDiagnosis">
        <rdf:type rdf:resource="http://www.mis.ugent.be/ontologies/ufo.owl#Quality_Universal"/>
    </owl:NamedIndividual>
    


    <!-- http://www.semanticweb.org/nalkhald/ontologies/2016/3/untitled-ontology-3#EmergencyDepartment -->

    <owl:NamedIndividual rdf:about="http://www.semanticweb.org/nalkhald/ontologies/2016/3/untitled-ontology-3#EmergencyDepartment">
        <rdf:type rdf:resource="http://www.mis.ugent.be/ontologies/ufo.owl#Base_Type"/>
    </owl:NamedIndividual>
    


    <!-- http://www.semanticweb.org/nalkhald/ontologies/2016/3/untitled-ontology-3#Examination -->

    <owl:NamedIndividual rdf:about="http://www.semanticweb.org/nalkhald/ontologies/2016/3/untitled-ontology-3#Examination">
        <rdf:type rdf:resource="http://www.mis.ugent.be/ontologies/ufo.owl#Relator_Universal"/>
    </owl:NamedIndividual>
    


    <!-- http://www.semanticweb.org/nalkhald/ontologies/2016/3/untitled-ontology-3#Examine_MedicalHistory -->

    <owl:NamedIndividual rdf:about="http://www.semanticweb.org/nalkhald/ontologies/2016/3/untitled-ontology-3#Examine_MedicalHistory">
        <rdf:type rdf:resource="http://www.mis.ugent.be/ontologies/ufo.owl#Event_Type"/>
    </owl:NamedIndividual>
    


    <!-- http://www.semanticweb.org/nalkhald/ontologies/2016/3/untitled-ontology-3#Examine_Symptoms -->

    <owl:NamedIndividual rdf:about="http://www.semanticweb.org/nalkhald/ontologies/2016/3/untitled-ontology-3#Examine_Symptoms">
        <rdf:type rdf:resource="http://www.mis.ugent.be/ontologies/ufo.owl#Event_Type"/>
    </owl:NamedIndividual>
    


    <!-- http://www.semanticweb.org/nalkhald/ontologies/2016/3/untitled-ontology-3#Fever -->

    <owl:NamedIndividual rdf:about="http://www.semanticweb.org/nalkhald/ontologies/2016/3/untitled-ontology-3#Fever">
        <rdf:type rdf:resource="http://www.mis.ugent.be/ontologies/ufo.owl#Quality_Universal"/>
    </owl:NamedIndividual>
    


    <!-- http://www.semanticweb.org/nalkhald/ontologies/2016/3/untitled-ontology-3#Headache -->

    <owl:NamedIndividual rdf:about="http://www.semanticweb.org/nalkhald/ontologies/2016/3/untitled-ontology-3#Headache">
        <rdf:type rdf:resource="http://www.mis.ugent.be/ontologies/ufo.owl#Quality_Universal"/>
    </owl:NamedIndividual>
    


    <!-- http://www.semanticweb.org/nalkhald/ontologies/2016/3/untitled-ontology-3#HealthCare -->

    <owl:NamedIndividual rdf:about="http://www.semanticweb.org/nalkhald/ontologies/2016/3/untitled-ontology-3#HealthCare">
        <rdf:type rdf:resource="http://www.mis.ugent.be/ontologies/ufo.owl#Relator_Universal"/>
    </owl:NamedIndividual>
    


    <!-- http://www.semanticweb.org/nalkhald/ontologies/2016/3/untitled-ontology-3#HeartAttack -->

    <owl:NamedIndividual rdf:about="http://www.semanticweb.org/nalkhald/ontologies/2016/3/untitled-ontology-3#HeartAttack">
        <rdf:type rdf:resource="http://www.mis.ugent.be/ontologies/ufo.owl#Quality_Universal"/>
        <rdfs:comment>Is the death of or damage to part of the 
heart muscle because the supply of blood 
to the heart muscle is severely reduced or stopped</rdfs:comment>
    </owl:NamedIndividual>
    


    <!-- http://www.semanticweb.org/nalkhald/ontologies/2016/3/untitled-ontology-3#HeartBeat -->

    <owl:NamedIndividual rdf:about="http://www.semanticweb.org/nalkhald/ontologies/2016/3/untitled-ontology-3#HeartBeat">
        <rdf:type rdf:resource="http://www.mis.ugent.be/ontologies/ufo.owl#Quality_Universal"/>
    </owl:NamedIndividual>
    


    <!-- http://www.semanticweb.org/nalkhald/ontologies/2016/3/untitled-ontology-3#Hospital -->

    <owl:NamedIndividual rdf:about="http://www.semanticweb.org/nalkhald/ontologies/2016/3/untitled-ontology-3#Hospital">
        <rdf:type rdf:resource="http://www.mis.ugent.be/ontologies/ufo.owl#Base_Type"/>
    </owl:NamedIndividual>
    


    <!-- http://www.semanticweb.org/nalkhald/ontologies/2016/3/untitled-ontology-3#IDCard -->

    <owl:NamedIndividual rdf:about="http://www.semanticweb.org/nalkhald/ontologies/2016/3/untitled-ontology-3#IDCard">
        <rdf:type rdf:resource="http://www.mis.ugent.be/ontologies/ufo.owl#Quality_Universal"/>
    </owl:NamedIndividual>
    


    <!-- http://www.semanticweb.org/nalkhald/ontologies/2016/3/untitled-ontology-3#MedicalFacility -->

    <owl:NamedIndividual rdf:about="http://www.semanticweb.org/nalkhald/ontologies/2016/3/untitled-ontology-3#MedicalFacility">
        <rdf:type rdf:resource="http://www.mis.ugent.be/ontologies/ufo.owl#Base_Type"/>
    </owl:NamedIndividual>
    


    <!-- http://www.semanticweb.org/nalkhald/ontologies/2016/3/untitled-ontology-3#MedicalHistory -->

    <owl:NamedIndividual rdf:about="http://www.semanticweb.org/nalkhald/ontologies/2016/3/untitled-ontology-3#MedicalHistory">
        <rdf:type rdf:resource="http://www.mis.ugent.be/ontologies/ufo.owl#Quality_Universal"/>
    </owl:NamedIndividual>
    


    <!-- http://www.semanticweb.org/nalkhald/ontologies/2016/3/untitled-ontology-3#MedicalInstitution -->

    <owl:NamedIndividual rdf:about="http://www.semanticweb.org/nalkhald/ontologies/2016/3/untitled-ontology-3#MedicalInstitution">
        <rdf:type rdf:resource="http://www.mis.ugent.be/ontologies/ufo.owl#Mixin_Type"/>
    </owl:NamedIndividual>
    


    <!-- http://www.semanticweb.org/nalkhald/ontologies/2016/3/untitled-ontology-3#Medication -->

    <owl:NamedIndividual rdf:about="http://www.semanticweb.org/nalkhald/ontologies/2016/3/untitled-ontology-3#Medication">
        <rdf:type rdf:resource="http://www.mis.ugent.be/ontologies/ufo.owl#Base_Type"/>
    </owl:NamedIndividual>
    


    <!-- http://www.semanticweb.org/nalkhald/ontologies/2016/3/untitled-ontology-3#Obtain_VitalSigns -->

    <owl:NamedIndividual rdf:about="http://www.semanticweb.org/nalkhald/ontologies/2016/3/untitled-ontology-3#Obtain_VitalSigns">
        <rdf:type rdf:resource="http://www.mis.ugent.be/ontologies/ufo.owl#Event_Type"/>
    </owl:NamedIndividual>
    


    <!-- http://www.semanticweb.org/nalkhald/ontologies/2016/3/untitled-ontology-3#Paramedics -->

    <owl:NamedIndividual rdf:about="http://www.semanticweb.org/nalkhald/ontologies/2016/3/untitled-ontology-3#Paramedics">
        <rdf:type rdf:resource="http://www.mis.ugent.be/ontologies/ufo.owl#Role_Type"/>
    </owl:NamedIndividual>
    


    <!-- http://www.semanticweb.org/nalkhald/ontologies/2016/3/untitled-ontology-3#Passport -->

    <owl:NamedIndividual rdf:about="http://www.semanticweb.org/nalkhald/ontologies/2016/3/untitled-ontology-3#Passport">
        <rdf:type rdf:resource="http://www.mis.ugent.be/ontologies/ufo.owl#Quality_Universal"/>
    </owl:NamedIndividual>
    


    <!-- http://www.semanticweb.org/nalkhald/ontologies/2016/3/untitled-ontology-3#Patient -->

    <owl:NamedIndividual rdf:about="http://www.semanticweb.org/nalkhald/ontologies/2016/3/untitled-ontology-3#Patient">
        <rdf:type rdf:resource="http://www.mis.ugent.be/ontologies/ufo.owl#Role_Type"/>
    </owl:NamedIndividual>
    


    <!-- http://www.semanticweb.org/nalkhald/ontologies/2016/3/untitled-ontology-3#PatientArrived -->

    <owl:NamedIndividual rdf:about="http://www.semanticweb.org/nalkhald/ontologies/2016/3/untitled-ontology-3#PatientArrived">
        <rdf:type rdf:resource="http://www.mis.ugent.be/ontologies/ufo.owl#Event_Type"/>
    </owl:NamedIndividual>
    


    <!-- http://www.semanticweb.org/nalkhald/ontologies/2016/3/untitled-ontology-3#PatientDetails -->

    <owl:NamedIndividual rdf:about="http://www.semanticweb.org/nalkhald/ontologies/2016/3/untitled-ontology-3#PatientDetails">
        <rdf:type rdf:resource="http://www.mis.ugent.be/ontologies/ufo.owl#Quality_Universal"/>
        <rdfs:comment>Any information relevant for the patient, such as name, age, etc</rdfs:comment>
    </owl:NamedIndividual>
    


    <!-- http://www.semanticweb.org/nalkhald/ontologies/2016/3/untitled-ontology-3#PatientDischarged -->

    <owl:NamedIndividual rdf:about="http://www.semanticweb.org/nalkhald/ontologies/2016/3/untitled-ontology-3#PatientDischarged">
        <rdf:type rdf:resource="http://www.mis.ugent.be/ontologies/ufo.owl#Event_Type"/>
    </owl:NamedIndividual>
    


    <!-- http://www.semanticweb.org/nalkhald/ontologies/2016/3/untitled-ontology-3#PatientRedirected -->

    <owl:NamedIndividual rdf:about="http://www.semanticweb.org/nalkhald/ontologies/2016/3/untitled-ontology-3#PatientRedirected">
        <rdf:type rdf:resource="http://www.mis.ugent.be/ontologies/ufo.owl#Event_Type"/>
    </owl:NamedIndividual>
    


    <!-- http://www.semanticweb.org/nalkhald/ontologies/2016/3/untitled-ontology-3#PediatricServices -->

    <owl:NamedIndividual rdf:about="http://www.semanticweb.org/nalkhald/ontologies/2016/3/untitled-ontology-3#PediatricServices">
        <rdf:type rdf:resource="http://www.mis.ugent.be/ontologies/ufo.owl#Relator_Universal"/>
    </owl:NamedIndividual>
    


    <!-- http://www.semanticweb.org/nalkhald/ontologies/2016/3/untitled-ontology-3#Perform_PhysicalExamination -->

    <owl:NamedIndividual rdf:about="http://www.semanticweb.org/nalkhald/ontologies/2016/3/untitled-ontology-3#Perform_PhysicalExamination">
        <rdf:type rdf:resource="http://www.mis.ugent.be/ontologies/ufo.owl#Event_Type"/>
    </owl:NamedIndividual>
    


    <!-- http://www.semanticweb.org/nalkhald/ontologies/2016/3/untitled-ontology-3#Perform_SurgicalExamination -->

    <owl:NamedIndividual rdf:about="http://www.semanticweb.org/nalkhald/ontologies/2016/3/untitled-ontology-3#Perform_SurgicalExamination">
        <rdf:type rdf:resource="http://www.mis.ugent.be/ontologies/ufo.owl#Event_Type"/>
    </owl:NamedIndividual>
    


    <!-- http://www.semanticweb.org/nalkhald/ontologies/2016/3/untitled-ontology-3#Person -->

    <owl:NamedIndividual rdf:about="http://www.semanticweb.org/nalkhald/ontologies/2016/3/untitled-ontology-3#Person">
        <rdf:type rdf:resource="http://www.mis.ugent.be/ontologies/ufo.owl#Base_Type"/>
    </owl:NamedIndividual>
    


    <!-- http://www.semanticweb.org/nalkhald/ontologies/2016/3/untitled-ontology-3#Pharmacy -->

    <owl:NamedIndividual rdf:about="http://www.semanticweb.org/nalkhald/ontologies/2016/3/untitled-ontology-3#Pharmacy">
        <rdf:type rdf:resource="http://www.mis.ugent.be/ontologies/ufo.owl#Base_Type"/>
    </owl:NamedIndividual>
    


    <!-- http://www.semanticweb.org/nalkhald/ontologies/2016/3/untitled-ontology-3#PhysicalExamination -->

    <owl:NamedIndividual rdf:about="http://www.semanticweb.org/nalkhald/ontologies/2016/3/untitled-ontology-3#PhysicalExamination">
        <rdf:type rdf:resource="http://www.mis.ugent.be/ontologies/ufo.owl#Relator_Universal"/>
    </owl:NamedIndividual>
    


    <!-- http://www.semanticweb.org/nalkhald/ontologies/2016/3/untitled-ontology-3#PhysicalTherapy -->

    <owl:NamedIndividual rdf:about="http://www.semanticweb.org/nalkhald/ontologies/2016/3/untitled-ontology-3#PhysicalTherapy">
        <rdf:type rdf:resource="http://www.mis.ugent.be/ontologies/ufo.owl#Relator_Universal"/>
    </owl:NamedIndividual>
    


    <!-- http://www.semanticweb.org/nalkhald/ontologies/2016/3/untitled-ontology-3#Physician -->

    <owl:NamedIndividual rdf:about="http://www.semanticweb.org/nalkhald/ontologies/2016/3/untitled-ontology-3#Physician">
        <rdf:type rdf:resource="http://www.mis.ugent.be/ontologies/ufo.owl#Role_Type"/>
    </owl:NamedIndividual>
    


    <!-- http://www.semanticweb.org/nalkhald/ontologies/2016/3/untitled-ontology-3#Prescription -->

    <owl:NamedIndividual rdf:about="http://www.semanticweb.org/nalkhald/ontologies/2016/3/untitled-ontology-3#Prescription">
        <rdf:type rdf:resource="http://www.mis.ugent.be/ontologies/ufo.owl#Base_Type"/>
        <rdfs:comment>A written formula for preparation and edministration of any remedy</rdfs:comment>
    </owl:NamedIndividual>
    


    <!-- http://www.semanticweb.org/nalkhald/ontologies/2016/3/untitled-ontology-3#PrescriptionProcessed -->

    <owl:NamedIndividual rdf:about="http://www.semanticweb.org/nalkhald/ontologies/2016/3/untitled-ontology-3#PrescriptionProcessed">
        <rdf:type rdf:resource="http://www.mis.ugent.be/ontologies/ufo.owl#Event_Type"/>
        <rdfs:comment>An event indicating that the prescription 
possessed by the pacient was processed 
by the pharmacist</rdfs:comment>
    </owl:NamedIndividual>
    


    <!-- http://www.semanticweb.org/nalkhald/ontologies/2016/3/untitled-ontology-3#PrescriptionReceived -->

    <owl:NamedIndividual rdf:about="http://www.semanticweb.org/nalkhald/ontologies/2016/3/untitled-ontology-3#PrescriptionReceived">
        <rdf:type rdf:resource="http://www.mis.ugent.be/ontologies/ufo.owl#Event_Type"/>
        <rdfs:comment>An event indicating receipt of medical prescription by the patient</rdfs:comment>
    </owl:NamedIndividual>
    


    <!-- http://www.semanticweb.org/nalkhald/ontologies/2016/3/untitled-ontology-3#Produce_DifferentialDiagnosis -->

    <owl:NamedIndividual rdf:about="http://www.semanticweb.org/nalkhald/ontologies/2016/3/untitled-ontology-3#Produce_DifferentialDiagnosis">
        <rdf:type rdf:resource="http://www.mis.ugent.be/ontologies/ufo.owl#Event_Type"/>
    </owl:NamedIndividual>
    


    <!-- http://www.semanticweb.org/nalkhald/ontologies/2016/3/untitled-ontology-3#Radiation -->

    <owl:NamedIndividual rdf:about="http://www.semanticweb.org/nalkhald/ontologies/2016/3/untitled-ontology-3#Radiation">
        <rdf:type rdf:resource="http://www.mis.ugent.be/ontologies/ufo.owl#Relator_Universal"/>
    </owl:NamedIndividual>
    


    <!-- http://www.semanticweb.org/nalkhald/ontologies/2016/3/untitled-ontology-3#Register_Patient -->

    <owl:NamedIndividual rdf:about="http://www.semanticweb.org/nalkhald/ontologies/2016/3/untitled-ontology-3#Register_Patient">
        <rdf:type rdf:resource="http://www.mis.ugent.be/ontologies/ufo.owl#Event_Type"/>
        <rdfs:comment>Adminstrative registers patient based 
on date provided by the patient</rdfs:comment>
    </owl:NamedIndividual>
    


    <!-- http://www.semanticweb.org/nalkhald/ontologies/2016/3/untitled-ontology-3#SpeachTherapy -->

    <owl:NamedIndividual rdf:about="http://www.semanticweb.org/nalkhald/ontologies/2016/3/untitled-ontology-3#SpeachTherapy">
        <rdf:type rdf:resource="http://www.mis.ugent.be/ontologies/ufo.owl#Relator_Universal"/>
    </owl:NamedIndividual>
    


    <!-- http://www.semanticweb.org/nalkhald/ontologies/2016/3/untitled-ontology-3#Surgeon -->

    <owl:NamedIndividual rdf:about="http://www.semanticweb.org/nalkhald/ontologies/2016/3/untitled-ontology-3#Surgeon">
        <rdf:type rdf:resource="http://www.mis.ugent.be/ontologies/ufo.owl#Role_Type"/>
    </owl:NamedIndividual>
    


    <!-- http://www.semanticweb.org/nalkhald/ontologies/2016/3/untitled-ontology-3#Surgery -->

    <owl:NamedIndividual rdf:about="http://www.semanticweb.org/nalkhald/ontologies/2016/3/untitled-ontology-3#Surgery">
        <rdf:type rdf:resource="http://www.mis.ugent.be/ontologies/ufo.owl#Relator_Universal"/>
    </owl:NamedIndividual>
    


    <!-- http://www.semanticweb.org/nalkhald/ontologies/2016/3/untitled-ontology-3#Symptoms -->

    <owl:NamedIndividual rdf:about="http://www.semanticweb.org/nalkhald/ontologies/2016/3/untitled-ontology-3#Symptoms">
        <rdf:type rdf:resource="http://www.mis.ugent.be/ontologies/ufo.owl#Quality_Universal"/>
    </owl:NamedIndividual>
    


    <!-- http://www.semanticweb.org/nalkhald/ontologies/2016/3/untitled-ontology-3#Therapy -->

    <owl:NamedIndividual rdf:about="http://www.semanticweb.org/nalkhald/ontologies/2016/3/untitled-ontology-3#Therapy">
        <rdf:type rdf:resource="http://www.mis.ugent.be/ontologies/ufo.owl#Relator_Universal"/>
    </owl:NamedIndividual>
    


    <!-- http://www.semanticweb.org/nalkhald/ontologies/2016/3/untitled-ontology-3#Trauma -->

    <owl:NamedIndividual rdf:about="http://www.semanticweb.org/nalkhald/ontologies/2016/3/untitled-ontology-3#Trauma">
        <rdf:type rdf:resource="http://www.mis.ugent.be/ontologies/ufo.owl#Quality_Universal"/>
    </owl:NamedIndividual>
    


    <!-- http://www.semanticweb.org/nalkhald/ontologies/2016/3/untitled-ontology-3#Treatment -->

    <owl:NamedIndividual rdf:about="http://www.semanticweb.org/nalkhald/ontologies/2016/3/untitled-ontology-3#Treatment">
        <rdf:type rdf:resource="http://www.mis.ugent.be/ontologies/ufo.owl#Relator_Universal"/>
    </owl:NamedIndividual>
    


    <!-- http://www.semanticweb.org/nalkhald/ontologies/2016/3/untitled-ontology-3#TriageNurse -->

    <owl:NamedIndividual rdf:about="http://www.semanticweb.org/nalkhald/ontologies/2016/3/untitled-ontology-3#TriageNurse">
        <rdf:type rdf:resource="http://www.mis.ugent.be/ontologies/ufo.owl#Role_Type"/>
    </owl:NamedIndividual>
    


    <!-- http://www.semanticweb.org/nalkhald/ontologies/2016/3/untitled-ontology-3#VitalSigns -->

    <owl:NamedIndividual rdf:about="http://www.semanticweb.org/nalkhald/ontologies/2016/3/untitled-ontology-3#VitalSigns">
        <rdf:type rdf:resource="http://www.mis.ugent.be/ontologies/ufo.owl#Quality_Universal"/>
    </owl:NamedIndividual>
</rdf:RDF>



<!-- Generated by the OWL API (version 3.4.2) http://owlapi.sourceforge.net -->

